

1. **Matrix Construction**: Let's denote your matrix as \( A = U^T U \), where \( U \) is an \( n \times m \) matrix.

2. **Compute the Inverse of \( U U^T \)**: First, compute the inverse (or pseudoinverse) of the smaller matrix \( U U^T \), which is an \( n \times n \) matrix:
   $$
   (U U^T)^{-1}
   $$

3. **Form the Pseudoinverse of \( A \)**: Using the relationship between \( A \) and \( U U^T \), the pseudoinverse of \( A \) can be constructed as:
   $$
   A^+ = (U^T U)^+ = U^+ (U^+)^T
   $$

4. **Compute the Pseudoinverse of \( U \)**: The pseudoinverse \( U^+ \) can be computed as:
   $$
   U^+ = U^T (U U^T)^{-1}
   $$

5. **Combine the Results**: Finally, combine the results to get the pseudoinverse of \( A \):
   $$
   A^+ = U^T (U U^T)^{-1} (U^T (U U^T)^{-1})^T = U^T (U U^T)^{-1} (U U^T)^{-1} U
   $$

By focusing on the smaller matrix \( U U^T \) and using the pseudoinverse, you can avoid dealing with the full matrix \( U^T U \) directly.

Here's the process in LaTeX:

1. **Matrix Construction**:
   $$
   A = U^T U
   $$

2. **Compute the Inverse of \( U U^T \)**:
   $$
   (U U^T)^{-1}
   $$

3. **Form the Pseudoinverse of \( A \)**:
   $$
   A^+ = (U^T U)^+ = U^+ (U^+)^T
   $$

4. **Compute the Pseudoinverse of \( U \)**:
   $$
   U^+ = U^T (U U^T)^{-1}
   $$

5. **Combine the Results**:
   $$
   A^+ = U^T (U U^T)^{-1} (U^T (U U^T)^{-1})^T = U^T (U U^T)^{-1} (U U^T)^{-1} U
   $$

This method leverages the structure of your matrix \( U \) and avoids dealing with the full matrix directly. If you need further clarification or a specific example, feel free to ask!
To find the \( n \times m \) matrix \( V \) such that \( V^T V = A^{-1} \), where \( A = U^T U \), you can follow these steps:

1. **Matrix Construction**: Recall that \( A = U^T U \).

2. **Compute the Pseudoinverse of \( U \)**: As previously mentioned, the pseudoinverse \( U^+ \) of \( U \) is:
   $$
   U^+ = U^T (U U^T)^{-1}
   $$

3. **Form the Pseudoinverse of \( A \)**: Using the pseudoinverse of \( U \), the pseudoinverse of \( A \) is:
   $$
   A^+ = (U^T U)^+ = U^+ (U^+)^T
   $$

4. **Identify the Matrix \( V \)**: To find the matrix \( V \) such that \( V^T V = A^{-1} \), we need to recognize that \( A^{-1} = (A^+)^{-1} \). Since \( A^+ = U^+ (U^+)^T \), we have:
   $$
   A^{-1} = (U^+ (U^+)^T)^{-1}
   $$

5. **Simplify the Expression**: Given that \( U^+ = U^T (U U^T)^{-1} \), we can write:
   $$
   A^{-1} = (U^T (U U^T)^{-1} (U^T (U U^T)^{-1})^T)^{-1}
   $$

6. **Find the Matrix \( V \)**: The matrix \( V \) can be identified as:
   $$
   V = (U U^T)^{-1/2} U
   $$

   This ensures that:
   $$
   V^T V = ((U U^T)^{-1/2} U)^T (U U^T)^{-1/2} U = U^T (U U^T)^{-1} U = A^{-1}
   $$

Here's the process in LaTeX:

1. **Matrix Construction**:
   $$
   A = U^T U
   $$

2. **Compute the Pseudoinverse of \( U \)**:
   $$
   U^+ = U^T (U U^T)^{-1}
   $$

3. **Form the Pseudoinverse of \( A \)**:
   $$
   A^+ = (U^T U)^+ = U^+ (U^+)^T
   $$

4. **Identify the Matrix \( V \)**:
   $$
   A^{-1} = (U^+ (U^+)^T)^{-1}
   $$

5. **Simplify the Expression**:
   $$
   A^{-1} = (U^T (U U^T)^{-1} (U^T (U U^T)^{-1})^T)^{-1}
   $$

6. **Find the Matrix \( V \)**:
   $$
   V = (U U^T)^{-1/2} U
   $$

   This ensures that:
   $$
   V^T V = ((U U^T)^{-1/2} U)^T (U U^T)^{-1/2} U = U^T (U U^T)^{-1} U = A^{-1}
   $$

By following these steps, you can find the \( n \times m \) matrix \( V \) whose crossproduct is \( A^{-1} \). If you need further clarification or a specific example, feel free to ask!
To compute the matrix square root, particularly for the matrix \( (U U^T) \), you can use the following approach:

1. **Eigenvalue Decomposition**: Perform the eigenvalue decomposition of \( U U^T \):
   $$
   U U^T = Q \Lambda Q^T
   $$
   where \( Q \) is an orthogonal matrix whose columns are the eigenvectors of \( U U^T \), and \( \Lambda \) is a diagonal matrix containing the eigenvalues of \( U U^T \).

2. **Square Root of Eigenvalues**: Compute the square root of each eigenvalue in \( \Lambda \) to form \( \Lambda^{1/2} \):
   $$
   \Lambda^{1/2} = \text{diag}(\sqrt{\lambda_1}, \sqrt{\lambda_2}, \ldots, \sqrt{\lambda_n})
   $$

3. **Form the Square Root Matrix**: Construct the square root matrix \( (U U^T)^{1/2} \) using the eigenvectors and the square roots of the eigenvalues:
   $$
   (U U^T)^{1/2} = Q \Lambda^{1/2} Q^T
   $$

4. **Inverse of the Square Root Matrix**: To find \( (U U^T)^{-1/2} \), invert the square root matrix:
   $$
   (U U^T)^{-1/2} = (Q \Lambda^{1/2} Q^T)^{-1} = Q (\Lambda^{1/2})^{-1} Q^T
   $$
   where \( (\Lambda^{1/2})^{-1} \) is the diagonal matrix with the reciprocals of the square roots of the eigenvalues:
   $$
   (\Lambda^{1/2})^{-1} = \text{diag}(1/\sqrt{\lambda_1}, 1/\sqrt{\lambda_2}, \ldots, 1/\sqrt{\lambda_n})
   $$

Here's the process in LaTeX:

1. **Eigenvalue Decomposition**:
   $$
   U U^T = Q \Lambda Q^T
   $$

2. **Square Root of Eigenvalues**:
   $$
   \Lambda^{1/2} = \text{diag}(\sqrt{\lambda_1}, \sqrt{\lambda_2}, \ldots, \sqrt{\lambda_n})
   $$

3. **Form the Square Root Matrix**:
   $$
   (U U^T)^{1/2} = Q \Lambda^{1/2} Q^T
   $$

4. **Inverse of the Square Root Matrix**:
   $$
   (U U^T)^{-1/2} = (Q \Lambda^{1/2} Q^T)^{-1} = Q (\Lambda^{1/2})^{-1} Q^T
   $$
   where:
   $$
   (\Lambda^{1/2})^{-1} = \text{diag}(1/\sqrt{\lambda_1}, 1/\sqrt{\lambda_2}, \ldots, 1/\sqrt{\lambda_n})
   $$

By following these steps, you can compute the matrix square root and its inverse, which will help you find the matrix \( V \) such that \( V^T V = A^{-1} \).


